Good progress on ghost task queue, now moving on to concrete task queue

share/steel/examples/pulse/parallel/GhostTaskQueue.fsti
@@ -6,7 +6,6 @@ module GR = Pulse.Lib.GhostReference
 
 open SingleGhostTask
 
-
 let rec is_same_mono_list (x y: mono_list) =
 match x, y with
 | [], [] -> True
@@ -14,6 +13,8 @@ match x, y with
 (*  tx._1 == ty._1 /\ tx._3 = ty._3 /\ tx._4 == ty._4 /\ tx._5 == ty._5 /\ is_same_mono_list qx qy *)
 same_extended_tasks tx ty /\ is_same_mono_list qx qy
 | _, _ -> False
+
+let x = ()
 
 let rec is_same_mono_same_length x y:
 Lemma (is_same_mono_list x y ==> L.length x = L.length y)
@@ -255,22 +256,6 @@ let recall_full #t #pos
 
 (** Part 3: Associated permissions: Reasoning done here **)
 
-module Lock = Pulse.Lib.SpinLock
-
-(*
-let task: Type u#1 = (
-  a: Type0 // return type of the computation
-  & r: ref (option a) // the reference where we put the result of the computation
-  & Lock.lock (own_res r)//(exists_ (fun v -> pts_to r half v ** (if None? v then pts_to r half v else emp)))
-  //& (unit_emp_stt_pure_pure a)
-  // to create this thing
-)
-
-let task_plus: Type u#1 = task_with_status task
-
-let mono_list_task_plus: Type u#1 = mono_list task
-*)
-
 let certificate (r:ghost_mono_ref) (t: task) (pos: nat)
 = M.witnessed r (task_in_queue t pos)
 
@@ -280,27 +265,48 @@ let get_certificate (t: task) (pos: nat)
             (l:mono_list)
             (_:squash (task_in_queue t pos l))
   : //TODO: SteelAtomicUT
-  stt_ghost (certificate r t pos)
+  stt_atomic (certificate r t pos) #Unobservable
+    emp_inames
                   (M.pts_to r full_perm l)
                   (fun _ -> M.pts_to r full_perm l)
-= witness r l _
-
-
-
-
-
-
-
+= admit()
+(* witness r l _ *)
 
 
 #pop-options
 
+(* TODO: Replace *)
+let alloc_M (#a:Type) (#p:Preorder.preorder a) (v:a)
+  : stt_atomic (M.ref a p) #Unobservable emp_inames emp (fun r -> M.pts_to r full_perm v)
+= admit()
+
+
+
 let inv_ghost_queue (r: ghost_mono_ref): vprop =
   exists* l. M.pts_to r one_half l ** tasks_res l
 
+(* 0: init queue *)
 ```pulse
-ghost
-fn add_todo_task (t: task) (l:mono_list)
+fn create_ghost_queue (_: unit)
+requires emp
+returns res: (r: ghost_mono_ref & inv (inv_ghost_queue r))
+ensures M.pts_to res._1 one_half []
+{
+
+  let r = alloc_M #_ #is_mono_suffix [];
+  M.share r full_perm [];
+  fold tasks_res [];
+  rewrite each (half_perm full_perm) as one_half;
+  fold inv_ghost_queue r;
+  let i: inv (inv_ghost_queue r) = new_invariant (inv_ghost_queue r);
+  let res: (r: ghost_mono_ref & inv (inv_ghost_queue r)) = Mkdtuple2 #_ #(fun r -> inv (inv_ghost_queue r)) r i;
+  rewrite each r as res._1;
+  res
+}
+```
+
+```pulse
+ghost fn add_todo_task (t: task) (l:mono_list)
   requires GR.pts_to t._1 #one_half true ** GR.pts_to t._2 #one_half false ** pts_to t._4 #one_half false ** GR.pts_to t._5 #one_half false
    ** tasks_res l
   ensures tasks_res (enqueue_todo l t)._1
@@ -312,6 +318,181 @@ fn add_todo_task (t: task) (l:mono_list)
 }
 ```
 
+```pulse
+unobservable fn add_todo_task_to_queue (r: ghost_mono_ref) (i: inv (inv_ghost_queue r)) (t: task)
+requires M.pts_to r one_half l ** GR.pts_to t._1 #one_half true ** GR.pts_to t._2 #one_half false ** pts_to t._4 #one_half false ** GR.pts_to t._5 #one_half false
+returns w: pos:nat & certificate r t pos
+ensures M.pts_to r one_half (enqueue_todo l t)._1
+opens (singleton i)
+{
+  with_invariants i {
+    unfold inv_ghost_queue r;
+    M.gather r one_half one_half l _;
+    let p = enqueue_todo l t;
+    let pos = p._2;
+    rewrite each (sum_perm one_half one_half) as full_perm;
+    M.write r p._1;
+    let w: certificate r t pos = get_certificate t pos r p._1 _;
+    add_todo_task t l;
+    M.share r full_perm _;
+    rewrite each (half_perm full_perm) as one_half;
+    fold inv_ghost_queue r;
+    let res = (| pos, w |);
+    res
+  }
+}
+```
+
+val assume_prop (p: prop): stt_ghost unit emp (fun () -> pure p)
+
+// 2: Pop
+```pulse
+ghost fn rec pop_task_from_todo_to_ongoing
+(l: mono_list{~(get_actual_queue l == [])})
+requires tasks_res l
+ensures tasks_res (pop_todo_task l)._2 ** 
+  GR.pts_to (pop_todo_task l)._1._1 #one_half true ** GR.pts_to (pop_todo_task l)._1._2 #one_half false ** ongoing_condition (pop_todo_task l)._1
+decreases l
+{
+  let et = L.hd l;
+  let q = L.tl l;
+  let p = pop_todo_task l;
+  rewrite (tasks_res l) as (task_res et ** tasks_res q);
+  if (et._2 = Todo) {
+    unfold task_res et;
+    from_todo_to_ongoing et;
+    rewrite (task_res (et._1, Ongoing) ** tasks_res q) as (tasks_res (pop_todo_task l)._2);
+    rewrite each et._1 as (pop_todo_task l)._1;
+    ()
+  }
+  else {
+    assert pure (get_actual_queue l == get_actual_queue (L.tl l));
+    pop_task_from_todo_to_ongoing (L.tl l);
+    rewrite each (pop_todo_task (L.tl l))._1 as (pop_todo_task l)._1;
+    rewrite (task_res et ** tasks_res (pop_todo_task (L.tl l))._2) as (tasks_res (pop_todo_task l)._2);
+    ()
+  }
+}
+```
+
+
+```pulse
+unobservable fn pop_task_ghost
+(r: ghost_mono_ref) (i: inv (inv_ghost_queue r)) (l: mono_list{~(get_actual_queue l == [])})
+  requires M.pts_to r one_half l 
+  returns pair:(pos:nat & certificate r (pop_todo_task l)._1 pos)
+  ensures M.pts_to r one_half (pop_todo_task l)._2 ** ongoing_condition (pop_todo_task l)._1 ** GR.pts_to (pop_todo_task l)._1._1 #one_half true ** GR.pts_to (pop_todo_task l)._1._2 #one_half false
+  opens (singleton i)
+{
+  with_invariants i {
+    unfold inv_ghost_queue r;
+    M.gather r one_half one_half l _;
+    rewrite each (sum_perm one_half one_half) as full_perm;
+    let p = pop_todo_task l;
+    let order_is_preserved = pop_preserves_order l;
+    M.write r p._2;
+    let w: certificate r p._1 p._3 = get_certificate p._1 p._3 r p._2 _;
+
+    rewrite each p._2 as (pop_todo_task l)._2;
+    pop_task_from_todo_to_ongoing l;
+
+    M.share r full_perm _;
+    rewrite each (half_perm full_perm) as one_half;
+    fold inv_ghost_queue r;
+    Mkdtuple2 #_ #(fun pos -> certificate r (pop_todo_task l)._1 pos) p._3 w
+  }
+}
+```
+
+// 3: From ongoing to todo: close_task
+
+let rec close_task_bis
+    (t: task)
+    (pos: nat)
+    (l: mono_list{task_in_queue t pos l /\ L.length l >= 1}):
+  mono_list
+= let (t', s)::q = l in
+if pos + 1 = L.length l
+  then (t', Done)::q // if s is not Ongoing, then we have too much permission
+  else (t', s)::(close_task_bis t pos q)
+
+let rec close_task_bis_preserves_order_aux
+    (t: task)
+    (pos: nat)
+    (l: mono_list{task_in_queue t pos l}):
+    Lemma (is_same_mono_list l (close_task_bis t pos l) )
+= match l with
+| (t', s)::q -> if pos + 1 = L.length l then is_mono_suffix_refl q
+else let q' = close_task_bis t pos q in close_task_bis_preserves_order_aux t pos q
+
+
+
+let close_task_bis_preserves_order
+    (t: task)
+    (pos: nat)
+    (l: mono_list{task_in_queue t pos l}):
+    Lemma (is_mono_suffix l (close_task_bis t pos l) )
+= close_task_bis_preserves_order_aux t pos l; from_same_to_suffix l (close_task_bis t pos l)
+
+(* updates the *done* reference, so not ghost or unobservable *)
+```pulse
+atomic fn rec close_task_from_ongoing_to_done
+(t: task) (pos: nat) (l: mono_list{task_in_queue t pos l})
+  requires GR.pts_to t._1 #one_half false ** GR.pts_to t._2 #one_half true ** ongoing_condition t ** (exists* v. pts_to t._4 #one_half v)
+    ** tasks_res l
+  //returns et:
+  ensures tasks_res (close_task_bis t pos l) ** pts_to t._4 #one_half true ** task_done t
+  decreases l
+{
+  rewrite tasks_res l as (task_res (L.hd l) ** tasks_res (L.tl l));
+  if (pos + 1 = L.length l)
+  {
+    let et = L.hd l;
+    assert task_res et ** pure (et._1 == t);
+    rewrite each t as et._1;
+
+    from_ongoing_to_done et;
+    rewrite (task_res (et._1, Done) ** tasks_res (L.tl l)) as tasks_res (close_task_bis t pos l);
+    rewrite each et._1 as t;
+    ()
+  }
+  else {
+    assert pure (pos + 1 < L.length l);
+    close_task_from_ongoing_to_done t pos (L.tl l);
+    rewrite (task_res (L.hd l) ** tasks_res (close_task_bis t pos (L.tl l))) as tasks_res (close_task_bis t pos l);
+    ()
+  }
+}
+```
+
+
+```pulse
+atomic fn conclude_task (t: task) (pos: nat)
+(r: ghost_mono_ref) (i: inv (inv_ghost_queue r))
+// (w: certificate r t pos) Needed to prove the refinement type
+(l: mono_list{task_in_queue t pos l})
+  requires M.pts_to r one_half l **
+    GR.pts_to t._1 #one_half false ** GR.pts_to t._2 #one_half true ** ongoing_condition t ** (exists* v. pts_to t._4 #one_half v)
+  ensures M.pts_to r one_half (close_task_bis t pos l) ** pts_to t._4 #one_half true ** task_done t
+  //M.pts_to r one_half (pop_todo_task l)._2 ** ongoing_condition (pop_todo_task l)._1 ** GR.pts_to (pop_todo_task l)._1._1 #one_half true ** GR.pts_to (pop_todo_task l)._1._2 #one_half false
+  opens (singleton i)
+{
+  with_invariants i {
+    unfold inv_ghost_queue r;
+    M.gather r one_half one_half l _;
+    rewrite each (sum_perm one_half one_half) as full_perm;
+    let p = close_task_bis t pos l;
+    let order_is_preserved = close_task_bis_preserves_order t pos l;
+    M.write r p;
+
+    close_task_from_ongoing_to_done t pos l;
+    M.share r full_perm _;
+    rewrite each (half_perm full_perm) as one_half;
+    fold inv_ghost_queue r;
+    ()
+  }
+}
+```
 (*
 Needed:
 0. Create ghost queue empty, invariant (with half permission)
@@ -324,722 +505,4 @@ We give back the other half
 3. We turn an ongoing task to todo
 
 4. We claim? We create the pledges?
-*)
-
-(* TD: Current progress here... *)
-
-(*
-// 1. create queue, alloc inv
-```pulse
-unobservable fn init_ghost_queue' (_: unit)
-requires emp
-returns res: (r:ghost_mono_ref & inv (inv_ghost_queue r))
-ensures M.pts_to res._1 one_half []
-{
-  let r = M.alloc #_ #is_mono_suffix [];
-
-  admit()
-  (*
-  let l: mono_list task = [(t, Todo)];
-  let r': M.ref (mono_list task) is_mono_suffix = M.alloc #emp_inames #_ (is_mono_suffix) l;
-  assert (M.pts_to r' full_perm l);
-  let r: gmref = convert_to_ghost_mono_ref r';
-
-  rewrite (M.pts_to r' full_perm l) as (M.pts_to r full_perm l);
-  let w: certificate r t 0 = get_certificate t 0 r l _;
-
-
-  let pair': (r:gmref & certificate r t 0) = (| r, w |);
-  let pair: erased (r:gmref & certificate r t 0) = hide pair';
-
-  share_queue r l;
-  assert (pure (count_ongoing l = 0 /\ get_actual_queue l == [t]));
-  // now: create tasks_res_own
-  //share pts_to t._2 #three_quart None
-  //share pts_to t._2
-  fold (task_res_own (t, Todo) three_quart);
-  rewrite emp as (tasks_res_own [] three_quart);
-  rewrite (task_res_own (t, Todo) three_quart ** tasks_res_own [] three_quart) as
-    (tasks_res_own l three_quart);
-  //fold (task_res_own t one_quart);
-  share_tasks_res_own l;
-  rewrite (M.pts_to r one_half l ** tasks_res_own l one_quart)
-    as `@(if 1 = 0 && L.length [t] = 0 then deadline r
-  else M.pts_to r one_half l ** tasks_res_own l one_quart);
-  fold small_inv r [t] 0;
-  rewrite (small_inv r [t] 0) as (small_inv (reveal pair)._1 [t] 0);
-  pair
-  *)
-}
-```
-
-let init_ghost_queue = init_ghost_queue'
-
-
-
-
-
-
-
-
-
-
-
-
-
-
-
-
-
-
-
-
-
-
-
-(*
-
-// assuming because of universe polymorphism
-assume val
-stt_return #a (x:a): stt a emp (fun y -> pure (x == y))
-
-// assuming because of universe polymorphism
-assume val
-stt_return_ghost #a (x:a): stt_ghost a emp_inames emp (fun y -> pure (x == y))
-*)
-
-
-
-#push-options "--print_universes --print_implicits"
-
-    
-
-
-
-(*
-```pulse
-ghost
-fn prove_task_ongoing_aux
-  (t: task)
-  (pos: nat)
-  (v: option t._1)
-  (l: (l:mono_list_task_plus{task_in_queue t pos l /\ L.length l >= 1}))
-  (f: hperm)
-//stt_ghost unit emp_inames
-requires tasks_res_own l f ** pts_to t._2 #three_quart v
-ensures tasks_res_own l f ** pts_to t._2 #three_quart v ** pure (count_ongoing l > 0)
-{
-  let h = L.hd l;
-  let q = L.tl l;
-
-  unfold (tasks_res_own l f);
-  rewrite `@(
-  match l with
-    | [] -> emp
-    | tl::ql -> task_res_own tl f ** tasks_res_own ql f)
-  as (task_res_own h f ** tasks_res_own q f);
-  assert (pts_to t._2 #three_quart v);
-  assert (task_res_own h f ** tasks_res_own q f);
-
-  if (pos + 1 = L.length l)
-  {
-    rewrite (pts_to (t._2) #three_quart v) as (pts_to (h._1._2) #three_quart v);
-    derive_status_ongoing h v f;
-    assert (pure (count_ongoing l > 0));
-    rewrite (pts_to (h._1._2) #three_quart v) as (pts_to (t._2) #three_quart v);
-    assert (pts_to t._2 #three_quart v);
-    fold_tasks_res_own h q f;
-    fold tasks_res_own l f;
-    ()
-  }
-  else {
-    prove_task_ongoing_aux_cb t pos v q f;
-    rewrite (task_res_own h f ** tasks_res_own q f) as
-      `@(match l with
-        | [] -> emp
-        | tl::ql -> task_res_own tl f ** tasks_res_own ql f);
-    fold (tasks_res_own l f);
-   ()
- }
-}
-```
-
-```pulse
-ghost
-fn prove_task_ongoing'
-  (#t: task)
-  (#pos: nat)
-  (#v: option t._1)
-  (r: gmref)
-  (q: list task) (c: int)
-  //(l: (l:mono_list task{task_in_queue t pos l /\ L.length l >= 1})):
-  (w:certificate r t pos)
-//stt_ghost unit emp_inames
-requires small_inv r q c ** pts_to t._2 #three_quart v
-ensures small_inv r q c ** pts_to t._2 #three_quart v ** pure (c > 0)
-{
-  unfold small_inv r q c;
-  with l. assert (M.pts_to r one_half l);
-  let proof = recall #task #t #pos r l w;
-  assert (pure (task_in_queue t pos l));
-  assert (pure (L.length l >= 1));
-  prove_task_ongoing_aux t pos v l one_half;
-  fold small_inv r q c;
-  ()
-}
-```
-//l
-
-(*
-  unfold is_active ct;
-  with v. assert (pts_to ct._1._2 #three_quart v);
-  prove_task_ongoing' #ct._1 #ct._2 #v r q c ct._3;
-  assert (pure (c > 0));
-  fold is_active ct;
-
-  unfold_small_inv r q c;
-
-*)
-
-let convert_to_ghost_mono_ref (r: M.ref (mono_list task) is_mono_suffix):
-  gmref
-  //ghost_mono_ref
-  = r
-
-  *)
-
-
-
-
-// 1: Enqueue
-```pulse
-ghost
-fn spawn_task_ghost'
-(r: gmref)
-(q: list task) (c: int) (t: task)
-(ct: current_task r)
-  requires small_inv r q c ** pts_to t._2 #three_quart None ** is_active ct
-  returns w: erased (pos:nat & certificate r t pos)
-  ensures small_inv r (t::q) c ** is_active ct
-{
-  unfold is_active ct;
-  with v. assert (pts_to ct._1._2 #three_quart v);
-  prove_task_ongoing' #ct._1 #ct._2 #v r q c ct._3;
-  assert (pure (c > 0));
-  fold is_active ct;
-
-  unfold_small_inv r q c;
-
-  with vl. assert (M.pts_to r full_perm vl);
-  assert (tasks_res_own vl three_quart);
-  assert (pure (count_ongoing vl = c /\ get_actual_queue vl == q));
-  let p = enqueue_todo #task vl t;
-  let pos = p._2;
-  assert (pure (task_in_queue t pos p._1));
-  write_ghost_queue #task #vl r p._1;
-  assert (M.pts_to r full_perm p._1);
-  let w: certificate r t pos = get_certificate t pos r p._1 _;
-  assert (tasks_res_own vl three_quart);
-  fold_done_task t vl three_quart;
-  assert (tasks_res_own (enqueue_todo vl t)._1 three_quart);
-  assert (M.pts_to r full_perm p._1);
-  rewrite (tasks_res_own (enqueue_todo vl t)._1 three_quart)
-    as (tasks_res_own p._1 three_quart);
-
-  fold_small_inv r (t::q) c;
-  //fold (small_inv r (t::q) c);
-  let res = hide (| pos, w |);
-  res
-}
-```
-
-let spawn_task_ghost = spawn_task_ghost'
-
-let rec vprop_equiv_test
-  (l: mono_list_task_plus{~(get_actual_queue l == [])}) (f: perm)
-: vprop_equiv (tasks_res_own l f)
-  (pts_to (pop_todo_task l)._1._2 #f None
-  ** tasks_res_own (pop_todo_task l)._2 f)
-= match l with
-| (t, Todo)::q ->
-let p1: vprop_equiv (tasks_res_own l f) 
-  (pts_to (pop_todo_task l)._1._2 #f None ** tasks_res_own q f) = vprop_equiv_refl _ in
-let p2: vprop_equiv (tasks_res_own q f) (emp ** tasks_res_own q f) = 
-  vprop_equiv_sym _ _ (vprop_equiv_unit _)
- in
-let p3: vprop_equiv (emp ** tasks_res_own q f) (tasks_res_own (pop_todo_task l)._2 f) = vprop_equiv_refl _ in
-let p4: vprop_equiv (tasks_res_own q f) (tasks_res_own (pop_todo_task l)._2 f) = vprop_equiv_trans _ _ _ p2 p3 in
-let p5 = vprop_equiv_cong _ _ _ _ (vprop_equiv_refl (pts_to (pop_todo_task l)._1._2 #f None)) p4 in
-vprop_equiv_trans _ _ _ p1 p5
-| t::q -> 
-let p1 = tasks_res_own l f in
-let p2 = task_res_own t f in
-let p3 = tasks_res_own q f in
-let p4 = pts_to (pop_todo_task q)._1._2 #f None in
-let p5 = tasks_res_own (pop_todo_task q)._2 f in
-let p6 = tasks_res_own (pop_todo_task l)._2 f in
-let e2: vprop_equiv p3 (p4 ** p5) = vprop_equiv_test q f in
-let e3: vprop_equiv p1 (p2 ** (p4 ** p5)) = vprop_equiv_cong p2 p3 p2 (p4 ** p5) (vprop_equiv_refl _) e2 in
-let e4: vprop_equiv (p2 ** (p4 ** p5)) ((p2 ** p4) ** p5) = vprop_equiv_sym _ _ (vprop_equiv_assoc _ _ _) in
-let e5: vprop_equiv ((p2 ** p4) ** p5) ((p4 ** p2) ** p5) = vprop_equiv_cong (p2 ** p4) p5 (p4 ** p2) p5
-  (vprop_equiv_comm _ _) (vprop_equiv_refl _) in
-let e6: vprop_equiv ((p4 ** p2) ** p5) (p4 ** (p2 ** p5)) = vprop_equiv_assoc _ _ _ in
-let e7: vprop_equiv (p2 ** (p4 ** p5)) (p4 ** (p2 ** p5)) = vprop_equiv_trans _ _ _ e4 (vprop_equiv_trans _ _ _ e5 e6)
-in vprop_equiv_trans _ _ _ e3 e7
-
-let get_permission_from_todo
-  (l: mono_list_task_plus{~(get_actual_queue l == [])}) (f:perm)
-: stt_ghost unit emp_inames
-(tasks_res_own l f)
-  (fun _ -> pts_to (pop_todo_task l)._1._2 #f None ** tasks_res_own (pop_todo_task l)._2 f)
-= rewrite _ _ (vprop_equiv_test l f)
-
-let mk_erased_pair #r #t (pos: nat) (w: certificate r t pos):
-  erased (pos: nat & certificate r t pos)
-= hide (|pos, w|)
-  //returns pair:erased (pos:nat & certificate r t pos)
-
-// 2: Pop
-```pulse
-ghost
-fn pop_task_ghost'
-(r: gmref)
-(t: task)
-(q: list task) (c: int)
-//(ct: current_task r)
-  requires small_inv r (t::q) c //** is_active ct
-  returns pair:erased (pos:nat & certificate r t pos)
-  ensures small_inv r q (c + 1) ** pts_to t._2 #three_quart None //** is_active ct
-{
-  //unfold is_active ct;
-  //with v. assert (pts_to ct._1._2 #three_quart v);
-  //prove_task_ongoing' #ct._1 #ct._2 #v r (t::q) c ct._3;
-  //assert (pure (c > 0));
-  //fold is_active ct;
-  unfold_small_inv r (t::q) c;
-
-  //unfold (small_inv r (t::q) c);
-  with l. assert (M.pts_to r full_perm l);
-  assert (tasks_res_own l three_quart);
-  assert (pure (count_ongoing l = c /\ get_actual_queue l == t::q));
-  let p = pop_todo_task #task l;
-  let order_is_preserved = pop_preserves_order #task l;
-  write_ghost_queue #task #l r p._2;
-  assert (M.pts_to r full_perm p._2);
-  let certif: certificate r t p._3 = get_certificate t p._3 r p._2 ();
-  assert (M.pts_to r full_perm p._2);
-  assert (pure (p._1 == t));
-  get_permission_from_todo l three_quart;
-  (*
-requires exists l. (M.pts_to r full_perm l
-  ** tasks_res_own l three_quart
-  ** pure (c = count_ongoing l /\ q == get_actual_queue l)
-  ** pure (c > 0)
-  )
-  *)
-  rewrite (tasks_res_own (pop_todo_task l)._2 three_quart)
-    as (tasks_res_own p._2 three_quart);
-  fold_small_inv r q (c + 1);
-  //fold (small_inv r q (c + 1));
-  rewrite (pts_to (pop_todo_task l)._1._2 #three_quart None)
-    as (pts_to t._2 #three_quart None);
-  let pair: erased (pos:nat & certificate r t pos) = mk_erased_pair p._3 certif;//(| p._3, certif |);
-  pair
-}
-```
-
-let pop_task_ghost = pop_task_ghost'
-
-let rec close_task_bis #a
-    (t: a)
-    (pos: nat)
-    (l: mono_list{task_in_queue t pos l /\ L.length l >= 1}):
-  mono_list
-= let (t', s)::q = l in
-if pos + 1 = L.length l
-  then (t', Done)::q // if s is not Ongoing, then we have too much permission
-  else (t', s)::(close_task_bis t pos q)
-
-let rec close_task_bis_preserves_order_aux #a
-    (t: a)
-    (pos: nat)
-    (l: mono_list{task_in_queue t pos l}):
-    Lemma (is_same_mono_list l (close_task_bis t pos l) )
-= match l with
-| (t', s)::q -> if pos + 1 = L.length l then is_mono_suffix_refl q
-else let q' = close_task_bis t pos q in close_task_bis_preserves_order_aux t pos q
-
-
-
-let close_task_bis_preserves_order #a
-    (t: a)
-    (pos: nat)
-    (l: mono_list{task_in_queue t pos l}):
-    Lemma (is_mono_suffix l (close_task_bis t pos l) )
-= close_task_bis_preserves_order_aux t pos l; from_same_to_suffix l (close_task_bis t pos l)
-
-
-```pulse
-ghost
-fn fold_task_done (h:(task & task_status)) (f: perm)
-  requires pts_to h._1._2 #f (Some x) ** pure (h._2 = Done)
-  ensures task_res_own h f
-{
-  assert (pts_to h._1._2 #f (Some x) ** pure (Some? (Some x)));
-  intro_exists (fun v -> pts_to h._1._2 #f v ** pure (Some? v)) (Some x);
-  rewrite (exists_ (fun v -> pts_to h._1._2 #f v ** pure (Some? v))) as (pts_to_Some h f);
-  rewrite (pts_to_Some h f) as (task_res_own h f);
-  ()
-}
-```
-
-// waiting to have recursion in Pulse
-assume val put_back_permission_cb
-  (t: task)
-  (pos: nat)
-  (l: (l:mono_list_task_plus{task_in_queue t pos l /\ L.length l >= 1}))
-  (x: t._1)
-:
-stt_ghost unit emp_inames
-(tasks_res_own l three_quart ** pts_to t._2 #three_quart (Some x))
-(fun () -> tasks_res_own (close_task_bis t pos l) three_quart ** pure (
- get_actual_queue (close_task_bis t pos l) == get_actual_queue l
-  /\ count_ongoing (close_task_bis t pos l) + 1 == count_ongoing l))
-
-```pulse
-ghost
-fn fold_tasks_res_own_bis
-  (h: (task & task_status)) 
-  (h': (task & task_status))
-  (q: mono_list_task_plus)
- (pos: nat) (t: task)
-(l: (l:mono_list_task_plus{task_in_queue t pos l /\ b2t (L.length l >= 1)}))
-requires task_res_own h' three_quart ** tasks_res_own q three_quart
-  ** pure (t == h._1 /\ h == L.hd l /\ q == L.tl l /\ h' == (h._1, Done)
-  /\ pos + 1 = L.length l
-  )
-  //** pure (t == h._1 /\ h == L.hd l /\ q == L.tl l)
-//ensures tasks_res_own (h::q) f
-ensures tasks_res_own (close_task_bis u#1 #task t pos l) three_quart
-{
-  rewrite (task_res_own h' three_quart ** tasks_res_own q three_quart) as (tasks_res_own (h'::q) three_quart);
-  rewrite (tasks_res_own (h'::q) three_quart)
-    as (tasks_res_own (close_task_bis u#1 #task t pos l) three_quart);
-  ()
-}
-```
-
-
-
-
-```pulse
-ghost
-fn put_back_permission
-  (t: task)
-  (pos: nat)
-  (l: (l:mono_list_task_plus{task_in_queue t pos l /\ L.length l >= 1}))
-  (x: t._1)
-requires tasks_res_own l three_quart ** pts_to t._2 #three_quart (Some x)
-ensures tasks_res_own (close_task_bis t pos l) three_quart ** pure (
- get_actual_queue (close_task_bis t pos l) == get_actual_queue l
-  /\ count_ongoing (close_task_bis t pos l) + 1 == count_ongoing l)
-{
-  let h = L.hd l;
-  let q = L.tl l;
-
-  unfold (tasks_res_own l three_quart);
-  rewrite `@(
-  match l with
-    | [] -> emp
-    | tl::ql -> task_res_own tl three_quart ** tasks_res_own ql three_quart)
-  as (task_res_own h three_quart ** tasks_res_own q three_quart);
-  assert (pts_to t._2 #three_quart (Some x));
-  assert (task_res_own h three_quart ** tasks_res_own q three_quart);
-
-  if (pos + 1 = L.length l)
-  {
-    assert (task_res_own h three_quart);
-    rewrite (pts_to (t._2) #three_quart (Some x)) as (pts_to (h._1._2) #three_quart (Some x));
-    derive_status_ongoing h (Some x) three_quart;
-    assert (pure (snd h = Ongoing));
-    assert (pts_to (h._1._2) #three_quart (Some x));
-
-    unfold (task_res_own h three_quart); // not needed, can be dropped
-    rewrite `@(match h._2 with
-      | Todo -> pts_to (h._1._2) #three_quart None
-      | Ongoing -> emp
-      | Done -> (exists_ (fun v -> pts_to (h._1._2) #three_quart v ** pure (Some? v))))
-    as (emp);
-
-    let h' = (h._1, Done);
-    rewrite (pts_to (h._1._2) #three_quart (Some x)) as (pts_to h'._1._2 #three_quart (Some x));
-    fold_task_done h' three_quart;
-    fold_tasks_res_own_bis h h' q pos t l;
-    assert (tasks_res_own (close_task_bis u#1 #task t pos l) three_quart);
-    ()
-
-  }
-  else {
-    put_back_permission_cb t pos q x;
-    assert (tasks_res_own (close_task_bis t pos q) three_quart);
-    assert (pure (get_actual_queue (close_task_bis t pos q) == get_actual_queue q));
-    assert (pure (get_actual_queue (close_task_bis t pos l) == get_actual_queue l));
-    assert (pure (count_ongoing (close_task_bis t pos q) + 1 == count_ongoing q));
-    assert (pure (count_ongoing (close_task_bis t pos l) + 1 == count_ongoing l));
-
-    rewrite (task_res_own h three_quart ** tasks_res_own (close_task_bis t pos q) three_quart) as
-    `@(
-    match (close_task_bis t pos l) with
-      | [] -> emp
-      | tl::ql -> task_res_own tl three_quart ** tasks_res_own ql three_quart);
-    fold (tasks_res_own (close_task_bis t pos l) three_quart);
-    ()
-  }
-}
-```
-
-let prove_task_ongoing = prove_task_ongoing'
-
-```pulse
-ghost
-fn prove_ongoing_non_neg'
-  (r:gmref)
-  (q: list task) (c: int)
-requires small_inv r q c
-ensures small_inv r q c ** pure (c >= 0)
-{
-  unfold small_inv r q c;
-  fold small_inv r q c;
-  ()
-}
-```
-
-// TODO
-let prove_ongoing_non_neg = prove_ongoing_non_neg'
-
-#push-options "--print_implicits --print_universes"
-
-// assume val assume_prop (p: prop): stt_ghost unit emp_inames emp (fun () -> pure p)
-
-(*
-```pulse
-ghost fn imp_false (b: bool) (p: vprop)
-  requires pure (b == false)
-  ensures imp_vprop b p
-{
-  rewrite emp as (imp_vprop b p);
-  ()
-}
-```
-
-```pulse
-ghost fn imp_true (b: bool) (p: vprop)
-  requires pure (b == true) ** p
-  ensures imp_vprop b p
-{
-  rewrite p as (imp_vprop b p);
-  ()
-}
-```
-*)
-
-
-assume val drop (p: vprop): stt_ghost unit emp_inames p (fun () -> emp)
-
-// 3: conclude the task
-```pulse
-ghost
-fn conclude_task_ghost'
-(#t: task)
-(#pos: nat)
-(r: gmref)
-(q: list task) (c: int)
-(x: t._1)
-(w: certificate r t pos)
-  requires small_inv r q c ** pts_to t._2 #three_quart (Some x)
-  ensures small_inv r q (c - 1) //** imp_vprop (c = 1 && L.length q = 0) (deadline r)
-{
-  prove_task_ongoing' #t #pos #(Some x) r q c w;
-  assert (pure (c > 0));
-  unfold_small_inv r q c;
-  //unfold (small_inv r q c);
-  with l. assert (M.pts_to r full_perm l);
-  assert (tasks_res_own l three_quart);
-  assert (pure (count_ongoing l = c /\ get_actual_queue l == q));
-  let proof = recall_full #task #t #pos r l w;
-  let p = close_task_bis t pos l;
-  let order_is_preserved = close_task_bis_preserves_order #task t pos l;
-  write_ghost_queue #task #l r p;
-  assert (M.pts_to r full_perm p);
-
-  put_back_permission t pos l x;
-  assert (tasks_res_own (close_task_bis t pos l) three_quart);
-
-  rewrite (tasks_res_own (close_task_bis u#1 #task t pos (reveal u#1 #(mono_list u#1 task) l)) three_quart)
-    as (tasks_res_own p three_quart);
-
-  assert (M.pts_to r full_perm p);
-  assert (pure (c - 1 = count_ongoing p /\ q == get_actual_queue p));
-
-  let b: bool = stt_ghost_reveal _ (c - 1 = 0 && L.length q = 0);
-  if (b)
-  {
-    share_queue r p;
-    share_tasks_res_own p;
-    obtain_deadline r one_quart;
-    duplicate_deadline r;
-
-    assert (M.pts_to r one_half p);
-    //assert (tasks_res_own p one_half ** tasks_res_own p one_quart);
-    rewrite (deadline r)
-      as `@(if c - 1 = 0 && L.length q = 0 then deadline r
-      else M.pts_to r one_half l ** tasks_res_own l one_quart);
-
-    assert (M.pts_to r one_half p **
-      tasks_res_own p one_half **
-      pure (count_ongoing p = c - 1 /\ get_actual_queue p == q)
-      ** `@(if c - 1 = 0 && L.length q = 0 then deadline r
-      else M.pts_to r one_half p ** tasks_res_own p one_quart));
-    fold (small_inv r q (c - 1));
-    //imp_true (c = 1 && L.length q = 0) (deadline r);
-    drop (deadline r);
-    ()
-  }
-  else {
-    fold_small_inv r q (c - 1);
-    //imp_false (c = 1 && L.length q = 0) (deadline r);
-    ()
-  }
-}
-```
-
-let conclude_task_ghost = conclude_task_ghost'
-
-let recall_certificate (#t: task) (#pos: nat)
-           (r:ghost_mono_ref)
-           (v: mono_list task)
-           (w:certificate r t pos)
-= recall_full r v w
-
-
-let pts_to_Some_fract (t:task) (f: perm): vprop
-= (exists_ (fun v -> pts_to t._2 #f v ** pure (Some? v)))
-
-// assuming recursion
-assume val get_Some_finished_aux_rec
-  (t: task) (pos: nat)
-  (l: mono_list_task_plus)
-  (f: perm)
-: stt_ghost unit emp_inames
-(tasks_res_own l f ** pure (task_in_queue t pos l) ** pure (count_ongoing l = 0 /\ get_actual_queue l == []))
-(fun _ -> tasks_res_own l (half_perm f) ** pts_to_Some_fract t (half_perm f))
-
-```pulse
-ghost
-fn get_Some_finished_aux
-  (t: task) (pos: nat)
-  (l: mono_list_task_plus)
-  (f: perm)
-requires tasks_res_own l f ** pure (task_in_queue t pos l)
-  ** pure (count_ongoing l = 0 /\ get_actual_queue l == [])
-//returns x: t._1
-//ensures tasks_res_own l f
-ensures tasks_res_own l (half_perm f) ** pts_to_Some_fract t (half_perm f)
-{
-  let h = L.hd l;
-  let q = L.tl l;
-
-  rewrite (tasks_res_own l f) as (task_res_own h f ** tasks_res_own q f);
-
-  if (pos + 1 = L.length l)
-  {
-    assert (task_res_own h f);
-    assert (pure (fst h == t));
-    assert (pure (snd h = Done));
-    rewrite (task_res_own h f) as (pts_to_Some h f);
-    unfold (pts_to_Some h f);
-    with y. assert (pts_to h._1._2 #f y);
-    share #_ #emp_inames h._1._2;
-    //rewrite (pts_to_Some h (half_perm f)) as (pts_to_Some_fract t (half_perm f));
-    //fold (pts_to_Some h (half_perm f));
-    (*
-fn fold_task_done (h:(task & task_status)) (f: perm)
-  requires pts_to h._1._2 #f (Some x) ** pure (h._2 = Done)
-  ensures task_res_own h f
-{
-  *)
-    with v. assert (pts_to h._1._2 #(half_perm f) v ** pure (Some? v));
-    //let x = Some?.v y;
-    assert (pure (Some (Some?.v v) == v));
-    rewrite (pts_to h._1._2 #(half_perm f) v) as (pts_to h._1._2 #(half_perm f) (Some (Some?.v v)));
-    rewrite (pts_to h._1._2 #(half_perm f) v) as (pts_to h._1._2 #(half_perm f) (Some (Some?.v v)));
-
-    //assert pts_to h._1._2 #f (Some x) ** pure (h._2 = Done)
-    fold_task_done h (half_perm f);
-    //fold (pts_to_Some_fract t (half_perm f));
-    //rewrite pts_to_Some h (half_perm f) as task_res_own h (half_perm f);
-    //assert (pts_to_Some h (half_perm f) ** pts_to_Some h (half_perm f));
-    //rewrite (pts_to_Some h (half_perm f)) as (task_res_own h (half_perm f));
-    share_tasks_res_own_general q f;
-    rewrite (task_res_own h (half_perm f) ** tasks_res_own q (half_perm f)) as (tasks_res_own l (half_perm f));
-    drop (tasks_res_own q (half_perm f));
-    //let x = Some?.v y;
-    //x
-    //unfold pts_to_Some h (half_perm f);
-    assert (pure (h._1 == t));
-    //with v. assert (pts_to h._1._2 #(half_perm f) v ** pure (Some? v));
-    rewrite (pts_to h._1._2 #(half_perm f) v ** pure (Some? v))
-      as (pts_to t._2 #(half_perm f) v ** pure (Some? v));
-    //rewrite (pts_to_Some h (half_perm f)) as (pts_to_Some_fract t (half_perm f));
-      //as (pts_to t._2 #(half_perm f) v ** pure (Some? v));
-    //intro_exists (fun v -> pts_to t._2 #(half_perm f) v ** pure (Some? v)) v;
-    fold pts_to_Some_fract t (half_perm f);
-    ()
-  }
-  else {
-    get_Some_finished_aux_rec t pos q f;
-    share_task_res_own h f;
-    rewrite (task_res_own h (half_perm f) ** tasks_res_own q (half_perm f))
-      as (tasks_res_own l (half_perm f));
-    drop (task_res_own h (half_perm f));
-    ()
-  }
-}
-```
-
-let recall_certificate_fract (#t: task) (#pos: nat)
-           (r:ghost_mono_ref)
-           (v: mono_list task)
-           (w:certificate r t pos)
-           (f: perm):
- stt_ghost unit emp_inames
-                 (M.pts_to r f v)
-                 (fun _ -> M.pts_to r f v ** pure (task_in_queue t pos v))
-  = M.recall (task_in_queue t pos) r v w
-
-
-
-```pulse
-ghost fn
-proof_promise' (#t: task) (#pos: nat)
-  (r: gmref)
-  (w:certificate r t pos)
-requires deadline r
-ensures deadline r ** (exists_ (fun f -> (exists_ (fun v ->
-                          pts_to t._2 #f v ** pure (Some? v)))))
-{
-  unfold deadline r;
-  with f1 f2 l. assert (M.pts_to r f1 l ** tasks_res_own l f2
-    ** pure (count_ongoing l = 0 /\ get_actual_queue l == []));
-  recall_certificate_fract r l w f1;
-  get_Some_finished_aux t pos l f2;
-  assert (tasks_res_own l (half_perm f2) ** pts_to_Some_fract t (half_perm f2));
-  fold deadline r;
-  unfold (pts_to_Some_fract t (half_perm f2));
-  ()
-}
-```
-
-let proof_promise = proof_promise'
-
 *)
